
伪代码示例：


```java
assert isEmpty(null)      = true
assert isEmpty("")        = true
assert isEmpty(" ")       = false
assert isEmpty("bob")     = false
assert isEmpty("  bob  ") = false
  
assert isBlank(null)      = true
assert isBlank("")        = true
assert isBlank(" ")       = true
assert isBlank("bob")     = false
assert isBlank("  bob  ") = false

assert equals(null, null)   = true
assert equals(null, "abc")  = false
assert equals("abc", null)  = false
assert equals("abc", "abc") = true
assert equals("abc", "ABC") = false

assert contains("abc", 'a')  = true
assert contains("abc", 'd')  = false
assert contains("abc", null) = false
assert contains(null, 'a')   = false
assert contains(null, null)  = false


assert join(null, *)         = null
assert join([], *)           = ""
assert join([null], *)       = ""
assert join([1, 2, 3], ';')  = "1;2;3"
assert join([1, 2, 3], null) = "123"

  
assert split(null, *)         = null
assert split("", *)           = []
assert split("abc def", null) = ["abc", "def"]
assert split("abc def", " ")  = ["abc", "def"]
assert split("abc  def", " ") = ["abc", "def"]
assert split("ab:cd:ef", ":") = ["ab", "cd", "ef"]


assert replace(null, *, *)       = null
assert replace("", *, *)         = ""
assert replace("any", null, *)   = "any"
assert replace("any", *, null)   = "any"
assert replace("any", "", *)     = "any"
assert replace("aba", "a", null) = "aba"
assert replace("aba", "a", "")   = "b"
assert replace("aba", "a", "z")  = "zbz"
```

```java
@Test  
public void isEmptyTest() {  
    assertTrue(isEmpty(null));  
    assertTrue(isEmpty(""));  
    assertFalse(isEmpty(" "));  
    assertFalse(isEmpty("bob"));  
    assertFalse(isEmpty(" bob "));  
}  
  
@Test  
public void isBank() {  
    assertTrue(isBlank(null));  
    assertTrue(isBlank(""));  
    assertTrue(isBlank(" "));  
    assertFalse(isBlank("bob"));  
    assertFalse(isBlank("  bob  "));  
}  
  
@Test  
public void containsTest() {  
    assertTrue(contains("abc", 'a'));  
    assertFalse(contains("abc", 'd'));  
    assertFalse(contains("abc", null));  
    assertFalse(contains(null, 'a'));  
    assertFalse(contains(null, null));  
}  
  
@Test  
public void joinTest() {  
    assertEquals(null, join((int[]) null, ','));  
    assertEquals("", join(new String[0], ','));  
    assertEquals("", join(Arrays.array((String) null), ','));  
    assertEquals("1;2;3", join(Arrays.array(1, 2, 3), ';'));  
    assertEquals("123", join(Arrays.array(1, 2, 3), null));  
}  
  
@Test  
public void splitTest() {  
    assertEquals(null, split(null, ','));  
    assertArrayEquals(new String[0], split("", ':'));  
    assertArrayEquals(Arrays.array("abc", "def"), split("abc def", null));  
    assertArrayEquals(Arrays.array("abc", "def"), split("abc def", " "));  
    assertArrayEquals(Arrays.array("abc", "def"), split("abc  def", " "));  
    assertArrayEquals(Arrays.array("ab", "cd", "ef"), split("ab:cd:ef", ":"));  
}  
  
@Test  
public void replaceTest() {  
    assertEquals(null, replace(null, "a", "b"));  
    assertEquals("", replace("", "a", "b"));  
    assertEquals("any", replace("any", null, "b") );  
    assertEquals("any", replace("any", "a", null));  
    assertEquals("any", replace("any", "", "b"));  
    assertEquals("aba", replace("aba", "a", null));  
    assertEquals("b", replace("aba", "a", ""));  
    assertEquals("zbz",replace("aba", "a", "z"));  
}
```
